rename

PsCore.v
@@ -13,7 +13,7 @@ Inductive term : Set :=
   | termcons : term
   | termpush : term
   | termexec : term
-  | termseq  : term -> term -> term.
+  | termpair : term -> term -> term.
 
 Definition stack : Set := list term.
 
@@ -31,16 +31,16 @@ Inductive eval : relation environment :=
       eval (t1 :: t2 :: vs, termswap :: ps) (t2 :: t1 :: vs, ps)
   | evalcons :
       forall (t1 t2 : term) (vs ps : stack),
-      eval (t1 :: t2 :: vs, termcons :: ps) (termseq t2 t1 :: vs, ps)
+      eval (t1 :: t2 :: vs, termcons :: ps) (termpair t2 t1 :: vs, ps)
   | evalpush :
       forall (t : term) (vs ps : stack),
       eval (vs, termpush :: t :: ps) (t :: vs, ps)
   | evalexec :
       forall (t : term) (vs ps : stack),
       eval (t :: vs, termexec :: ps) (vs, t :: ps)
-  | evalseq  :
+  | evalpair  :
       forall (t1 t2 : term) (vs ps : stack),
-      eval (vs, termseq t1 t2 :: ps) (vs, t1 :: t2 :: ps).
+      eval (vs, termpair t1 t2 :: ps) (vs, t1 :: t2 :: ps).
 
 Definition evalrtc : relation environment := clos_refl_trans _ eval.
 Definition evalrtc' : relation environment := clos_refl_trans_1n _ eval.
@@ -49,7 +49,8 @@ Infix "|=>" := eval (at level 80, no associativity).
 Infix "|=>*" := evalrtc (at level 80, no associativity).
 Infix "|=>*'" := evalrtc' (at level 80, no associativity).
 
-Lemma evalrtc_is_evalrtc' : forall (e1 e2 : environment), e1 |=>* e2 <-> e1 |=>*' e2.
+Lemma evalrtc_is_evalrtc' :
+  forall (e1 e2 : environment), e1 |=>* e2 <-> e1 |=>*' e2.
   intros ; split ; [ apply clos_rt_rt1n | apply clos_rt1n_rt ].
 Qed.
 
@@ -84,7 +85,7 @@ Lemma decide_eval : forall (e1 : environment),
   destruct s.
   right ; intro ; destruct H ; inversion H.
   left ; eexists ; apply evalexec.
-  left ; eexists ; apply evalseq.
+  left ; eexists ; apply evalpair.
 Defined.
 
 Lemma eval_unique : forall (a b c : environment), a |=> b -> a |=> c -> b = c.
@@ -127,7 +128,6 @@ Ltac evalstep' e1 e2 :=
   match eval hnf in (decide_eval e1) with
     | or_introl _ (ex_intro _ ?e3 ?p) =>
       apply (rt_trans _ _ _ _ _ (rt_step _ _ _ _ p))
-    | or_intror _ _ => idtac
     | _ => idtac
   end.
 
@@ -152,58 +152,58 @@ Ltac rtcequal :=
     | _ => fail 2 "The goal is invalid."
   end.
 
-Definition termnop : term := termseq (termseq termpush termpop) termpop.
+Definition termnop : term := termpair (termpair termpush termpop) termpop.
 
 Lemma evalnop : forall (vs ps : stack), (vs, termnop :: ps) |=>* (vs, ps).
   intros ; evalauto.
 Qed.
 
-Definition termlist' : list term -> term -> term := fold_left termseq.
+Definition termseq' : list term -> term -> term := fold_left termpair.
 
-Lemma eval_termlist' : forall (ts : list term) (t : term) (vs ps : stack),
-  (vs, termlist' ts t :: ps) |=>* (vs, t :: ts ++ ps).
+Lemma eval_termseq' : forall (ts : list term) (t : term) (vs ps : stack),
+  (vs, termseq' ts t :: ps) |=>* (vs, t :: ts ++ ps).
   induction ts ; intros.
   evalauto.
   evalpartial IHts ; evalauto.
 Qed.
 
-Definition termlist (ts : list term) : term := termlist' ts termnop.
+Definition termseq (ts : list term) : term := termseq' ts termnop.
 
-Lemma eval_termlist : forall (ts : list term) (vs ps : stack),
-  (vs, termlist ts :: ps) |=>* (vs, ts ++ ps).
+Lemma eval_termseq : forall (ts : list term) (vs ps : stack),
+  (vs, termseq ts :: ps) |=>* (vs, ts ++ ps).
   intros.
-  evalpartial eval_termlist'.
+  evalpartial eval_termseq'.
   evalauto.
 Qed.
 
-Lemma termlist_replicate : forall (n : nat) (t1 t2 : term),
-  termlist' (replicate n t1) t2 =
-    fold_right (flip termseq) t2 (replicate n t1).
+Lemma termseq_replicate : forall (n : nat) (t1 t2 : term),
+  termseq' (replicate n t1) t2 =
+    fold_right (flip termpair) t2 (replicate n t1).
   intros.
   rewrite (replicate_rev_id n t1) at 2.
-  apply (eq_sym (fold_left_rev_right (flip termseq) (replicate n t1) t2)).
+  apply (eq_sym (fold_left_rev_right (flip termpair) (replicate n t1) t2)).
 Qed.
 
-Lemma app_termlist' : forall (ts1 ts2 : list term) (t : term),
-  termlist' (ts1 ++ ts2) t = termlist' ts2 (termlist' ts1 t).
+Lemma app_termseq' : forall (ts1 ts2 : list term) (t : term),
+  termseq' (ts1 ++ ts2) t = termseq' ts2 (termseq' ts1 t).
   intros ; apply fold_left_app.
 Qed.
 
-Lemma app_termlist : forall (ts1 ts2 : list term),
-  termlist (ts1 ++ ts2) = termlist' ts2 (termlist ts1).
-  intros ; apply app_termlist'.
+Lemma app_termseq : forall (ts1 ts2 : list term),
+  termseq (ts1 ++ ts2) = termseq' ts2 (termseq ts1).
+  intros ; apply app_termseq'.
 Qed.
 
-Definition termsnoc : term := termlist [ termswap ; termcons ].
+Definition termsnoc : term := termseq [ termswap ; termcons ].
 
 Lemma evalsnoc : forall (t1 t2 : term) (vs ps : stack),
-  (t1 :: t2 :: vs, termsnoc :: ps) |=>* (termseq t1 t2 :: vs, ps).
+  (t1 :: t2 :: vs, termsnoc :: ps) |=>* (termpair t1 t2 :: vs, ps).
   intros ; evalauto.
 Qed.
 
-Definition termquote : term := termlist [termpush ; termpush ; termsnoc ].
+Definition termquote : term := termseq [termpush ; termpush ; termsnoc ].
 
 Lemma eval_termquote : forall (t : term) (vs ps : stack),
-  (t :: vs, termquote :: ps) |=>* (termseq termpush t :: vs, ps).
+  (t :: vs, termquote :: ps) |=>* (termpair termpush t :: vs, ps).
   intros ; evalauto.
 Qed.
